src/Spec/Proc.v
@@ -1,3 +1,5 @@
+Require Import Helpers.ProofAutomation.
+
 Global Set Implicit Arguments.
 
 Section Proc.
@@ -13,6 +15,39 @@ Section Proc.
        | Atomic (p:proc)
   .
 
+  Fixpoint seq (p1 p2: proc) : proc :=
+    match p1 with
+    | Ret => p2
+    | Exec a p' => Exec a (seq p' p2)
+    end.
+
+  Infix ";;" := seq (at level 14).
+
+  Theorem seq_assoc : forall p1 p2 p3,
+      p1;; p2;; p3 = p1;; (p2;; p3).
+  Proof.
+    induct p1; simpl; congruence.
+  Qed.
+
+  Definition seq_ret_l p :
+      Ret;; p = p := eq_refl.
+
+  Theorem seq_ret_r : forall p,
+      p;; Ret = p.
+  Proof.
+    induct p; simpl; congruence.
+  Qed.
+
 End Proc.
 
 Arguments proc Op : clear implicits.
+
+Notation "p1 ;; p2" := (seq p1 p2) (at level 14, left associativity,
+                                    format "p1 ;;  '/' p2").
+
+Notation "a ~ p" := (Exec a p) (at level 13, right associativity).
+
+(* printing test *)
+Local Definition example Op (o:Op) : proc Op :=
+  Call o ~ Call o ~ Ret;;
+                     Spawn (Call o ~ Ret) ~ Ret.
