src/Spec/TraceIncl.v
@@ -1,5 +1,12 @@
 Require Import Spec.Proc.
 Require Import Spec.Exec.
+Require Import Spec.ThreadsState.
+
+Require Import Helpers.ProofAutomation.
+Require Import Helpers.TransitionSystem.
+
+Require Import List.
+Import ListNotations.
 
 Section Semantics.
   Variable Op:Type.
@@ -15,5 +22,38 @@ Section Semantics.
     forall s s' tr tr' ts1',
       exec (ts [[tid := p1]], s, tr) (ts1', s', tr') ->
       exists ts2', exec (ts [[tid := p2]], s, tr) (ts2', s', tr').
+
+  Ltac exec_step_inv H :=
+    lazymatch type of H with
+    | exec_step _ _ ?ss =>
+      ((is_var ss; let ts := fresh "ts" in
+                  let s := fresh "s" in
+                  let tr := fresh "tr" in
+                  destruct ss as ((ts & s) & tr)) || idtac);
+      apply exec_step_inv in H;
+      destruct H;
+      propositional
+    end.
+
+  Theorem atomic_trace_incl : forall p p',
+      trace_incl (Exec (Atomic p) p') (p;; p').
+  Proof.
+    unfold trace_incl; intros.
+    match goal with
+    | [ H: exec ?ss ?ss' |- _ ] =>
+      remember ss as ss1;
+        remember ss' as ss2
+    end.
+    generalize dependent ts.
+    generalize dependent ts1'.
+    induct H.
+    - repeat match goal with
+             | [ H: (_, _) = (_, _) |- _ ] => invert H; clear H
+             end.
+      eexists; reflexivity.
+    - specialize (IHkleene_star _ eq_refl).
+      exec_step_inv H.
+      (* TODO: can construct executions for a whole list of actions *)
+  Abort.
 
 End Semantics.
